theories/Hoare.v
@@ -118,7 +118,7 @@ Section CANCEL.
 
   Variable entry_r: Σ.
   Variable mainpre: Any.t -> ord -> Σ -> Prop.
-  Variable (mainbody: list val -> itree (hCallE +' pE +' eventE) val).
+  Variable (mainbody: Any.t -> itree (hCallE +' pE +' eventE) Any.t).
   Hypothesis MAINPRE: mainpre ([]: list val)↑ ord_top entry_r.
 
   Hypothesis WFR: URA.wf (entry_r ⋅ rsum (ModSemL.initial_r_state ms_tgt)).
@@ -183,7 +183,7 @@ Section CANCEL.
 
   Variable entry_r: Σ.
   Variable mainpre: Any.t -> ord -> Σ -> Prop.
-  Variable (mainbody: list val -> itree (hCallE +' pE +' eventE) val).
+  Variable (mainbody: Any.t -> itree (hCallE +' pE +' eventE) Any.t).
   Hypothesis MAINPRE: mainpre ([]: list val)↑ ord_top entry_r.
 
   Hypothesis WFR: URA.wf (entry_r ⋅ rsum (ModSemL.initial_r_state ms_tgt)).
